Remove dependency on computability/lambda and recfunsTheory
Needs some reworking of proofs because of the automatic rewrite
DISJ_IMP_EQ from churchDBTheory. Eventually move this theorem into the
primeq script so that its goodness can continue to be used. (Very
tempted to move the whole thing somewhere more global.)

examples/computability/turingMachines/turing_machineScript.sml
@@ -1,7 +1,4 @@
-
-
 open HolKernel Parse boolLib bossLib finite_mapTheory;
-open recfunsTheory;
 open recursivefnsTheory;
 open prnlistTheory;
 open primrecfnsTheory;
@@ -12,7 +9,6 @@ open pred_setTheory;
 val _ = new_theory "turing_machine";
 
 val _ = intLib.deprecate_int()
-
 
 (*
 Li and Vitayi book
@@ -73,10 +69,10 @@ val _ = Datatype `cell = Z | O `;
 val _ = Datatype `state = <| n : num |>`;
 
 val _ = Datatype `TM = <| state : state;
-                  prog : ((state # cell) |->  (state # action));
-                  tape_l : cell list;
-                  tape_h : cell;
-                  tape_r : cell list
+                          prog : ((state # cell) |->  (state # action));
+                          tape_l : cell list;
+                          tape_h : cell;
+                          tape_r : cell list
                        |>`;
 
 val concatWith_def = Define`
@@ -84,50 +80,46 @@ val concatWith_def = Define`
   (concatWith sep [x] = x) /\
   (concatWith sep (x::y::rest) = x ++ sep ++ concatWith sep (y::rest))`;
 
-EVAL ``concatWith [0n] [[1;2;3;4]; [4;5]; [10;11;13]]``;
-
-EVAL ``GENLIST (K O) 24 ``;
-
-val INITIAL_TAPE_TM_def = Define `(INITIAL_TAPE_TM tm [] = tm) ∧
-  (INITIAL_TAPE_TM tm (h::t) = tm with <|tape_l := [] ; tape_h := h ; tape_r := t|>)`;
+val INITIAL_TAPE_TM_def = Define `
+  (INITIAL_TAPE_TM tm [] = tm) ∧
+  (INITIAL_TAPE_TM tm (h::t) =
+    tm with <|tape_l := [] ; tape_h := h ; tape_r := t|>)
+`;
 
 val INITIAL_TM_def = Define`
-INITIAL_TM p args =
-INITIAL_TAPE_TM <|state := <|n:=0|>;  prog := p;tape_l := [];tape_h := Z;tape_r := []|> (concatWith [Z] (MAP (GENLIST (K O)) args ))`;
-
-EVAL ``INITIAL_TM FEMPTY [2;3]``;
+  INITIAL_TM p args =
+    INITIAL_TAPE_TM <| state := <|n:=0|>;  prog := p;tape_l := [];
+                       tape_h := Z;tape_r := [] |>
+                    (concatWith [Z] (MAP (GENLIST (K O)) args))`;
 
 val UPDATE_STATE_TIME = Define `UPDATE_STATE_TIME tm =
-  if(((tm.state),(tm.tape_h)) IN FDOM tm.prog)
-  then tm with
-    <|state := (FST (tm.prog ' ((tm.state) ,(tm.tape_h)) )) |>
-    else (tm)
+  if (tm.state,tm.tape_h) IN FDOM tm.prog
+  then tm with <|state := (FST (tm.prog ' ((tm.state) ,(tm.tape_h)) )) |>
+  else (tm)
                                `;
 
-val UPDATE_TAPE_def = Define `UPDATE_TAPE tm =
-  if (((tm.state),(tm.tape_h)) IN FDOM tm.prog) ∧ (tm.state.n <> 0)
-  then let tm' = tm with
-    <|    state := (FST (tm.prog ' ((tm.state) ,(tm.tape_h)) )) |> in
-      case (SND (tm.prog ' ((tm.state) ,(tm.tape_h)) )) of
-        Wr0 => tm' with tape_h := Z
-      | Wr1 => tm' with tape_h := O
-      | L   => if (tm.tape_l = [])
-        then tm' with <| tape_l := [];
-                        tape_h := Z ;
-                        tape_r := tm.tape_h::tm.tape_r |>
-        else tm' with <| tape_l := TL tm.tape_l;
-           tape_h := HD tm.tape_l ;
-           tape_r := tm.tape_h::tm.tape_r |>
-       | R   => if (tm.tape_r = [])
-         then tm' with <| tape_l := tm.tape_h::tm.tape_l;
-           tape_h := Z ;
-           tape_r := [] |>
-         else tm' with <| tape_l := tm.tape_h::tm.tape_l;
-           tape_h := HD tm.tape_r;
-           tape_r := TL tm.tape_r |>
-  else (tm with state := <|n:=0|> )
-                                  `;
-
+val UPDATE_TAPE_def = Define `
+  UPDATE_TAPE tm =
+    if (tm.state,tm.tape_h) IN FDOM tm.prog ∧ tm.state.n <> 0 then
+      let tm' = tm with state := FST (tm.prog ' ((tm.state) ,(tm.tape_h)) )
+      in
+        case SND (tm.prog ' (tm.state ,tm.tape_h)) of
+          Wr0 => tm' with tape_h := Z
+        | Wr1 => tm' with tape_h := O
+        | L   => if (tm.tape_l = [])
+                 then tm' with <| tape_l := []; tape_h := Z ;
+                                  tape_r := tm.tape_h::tm.tape_r |>
+                 else tm' with <| tape_l := TL tm.tape_l;
+                                  tape_h := HD tm.tape_l ;
+                                  tape_r := tm.tape_h::tm.tape_r |>
+        | R   => if (tm.tape_r = []) then
+                  tm' with <| tape_l := tm.tape_h::tm.tape_l; tape_h := Z;
+                              tape_r := [] |>
+                 else tm' with <| tape_l := tm.tape_h::tm.tape_l;
+                                  tape_h := HD tm.tape_r;
+                                  tape_r := TL tm.tape_r |>
+    else tm with state := <|n:=0|>
+`;
 
 val _ = overload_on("RUN",``FUNPOW UPDATE_TAPE``);
 
@@ -198,30 +190,6 @@ val DIV_3_lem = Q.store_thm(
                   >> `4 DIV 3 <= (n' +4) DIV 3` by metis_tac[DIV_LE_MONOTONE]
                   >> `1 <=0` by fs[]
                   >> fs[]
-    );
-
-
-val MOD_3_lem = Q.store_thm (
-        "MOD_3_lem",
-`∀ n. (n MOD 3 = 0) ∨ (n MOD 3 = 1) ∨ (n MOD 3 = 2)`,
-Induct_on `n` >- fs[] >> rw[] >> `SUC n MOD 3 < 3` by fs[] >> `1 < SUC n MOD 3` by fs[]
-          >> `2 <=  SUC n MOD 3` by fs[]
-          >> `0<3` by fs[] >> `SUC n MOD 3 <= SUC n` by metis_tac[MOD_LESS_EQ]
-          >> `SUC n MOD 3 < 2 + 1` by fs[]
-          >> `SUC n MOD 3 <= 2` by metis_tac[LE_LT1]
-          >> fs[]
-    );
-
-
-val MOD_DIV_3_lem = Q.store_thm(
-        "MOD_DIV_3_lem",
-`∀ n. ((n DIV 3 = 0) ∧ (n MOD 3 = 0)) ==> (n = 0)`,
-Induct_on `n` >- fs[]
-          >> rw[] >> `SUC n = n+1` by fs[] >> CCONTR_TAC >> fs[] >> rw[]
-          >> `SUC n DIV 3 = SUC n MOD 3` by fs[]
-          >> `SUC n < 3` by metis_tac[DIV_3_lem]
-          >> `SUC n = 0` by fs[]
-          >> fs[]
     );
 
 
@@ -513,20 +481,6 @@ val WRITE_1_HEAD_lem = Q.store_thm("WRITE_1_HEAD_lem",
 `∀ tm s. (UPDATE_ACT_S_TM s Wr1 tm).tape_h = O`,
 rpt strip_tac >> rw[UPDATE_ACT_S_TM_def] );
 
-
-val TMN_Z_MOD_1_lem = Q.store_thm ("TMN_Z_MOD_1_lem",
-`∀ tmn. ((nfst (nsnd tmn) MOD 2 = 1) ∧ (HD (FST (DECODE_TM_TAPE (nsnd tmn))) = Z)) <=> F`,
-strip_tac >> rw[]  >> `~(nfst (nsnd tmn) MOD 2 = 0)` by fs[] >>
-`~EVEN (nfst (nsnd tmn))` by metis_tac[EVEN_MOD2] >>
-`ODD (nfst (nsnd tmn))` by metis_tac[EVEN_OR_ODD] >>
-`EVEN 0` by fs[] >>
-`~((nfst (nsnd tmn)) = 0)` by metis_tac[EVEN_OR_ODD] >>
-Cases_on `nfst (nsnd tmn)` >- fs[] >> 
-`DECODE (SUC n) = [O] ++ (DECODE (((SUC n) - 1) DIV 2))` by fs[DECODE_def] >>
-`TL (DECODE (SUC n)) = (DECODE ((SUC n -1) DIV 2))` by fs[DECODE_def] >>
-rw[] >> rw[DECODE_TM_TAPE_def] );
-
-
 val ODD_TL_DECODE_lem = Q.store_thm ("ODD_TL_DECODE_lem",
 `∀ n. (ODD n) ==> (TL (DECODE n) = DECODE ((n-1) DIV 2))`,
 rpt strip_tac >> `EVEN 0` by EVAL_TAC >> `~(n = 0)` by metis_tac[EVEN_AND_ODD]>>
@@ -688,13 +642,13 @@ Induct_on `p` >> simp[] )
 val nfst_lem = Q.store_thm("nfst_lem",
 `(∀n. P (nfst n)) ==> (∀k. P k)`,
 strip_tac >> Induct_on `k` >- (`nfst 0 = 0` by EVAL_TAC >> `P (nfst 0)` by fs[]>> metis_tac[] )
-          >- (`∃l j. nfst (l *, j)= SUC k` by fs[nfst_npair] >> 
+          >- (`∃l j. nfst (l *, j)= SUC k` by fs[nfst_npair] >>
 `P (nfst (l *, j)) ` by rfs[]  >>  metis_tac[]  ) );
 
 val nsnd_lem = Q.store_thm("nfst_lem",
 `(∀n. P (nsnd n)) ==> (∀k. P k)`,
 strip_tac >> Induct_on `k` >- (`nsnd 0 = 0` by EVAL_TAC >> `P (nsnd 0)` by fs[]>> metis_tac[] )
-          >- (`∃l j. nsnd (l *, j)= SUC k` by fs[nsnd_npair] >> 
+          >- (`∃l j. nsnd (l *, j)= SUC k` by fs[nsnd_npair] >>
 `P (nsnd (l *, j)) ` by rfs[]  >>  metis_tac[]  ) );
 
 val nfst_nsnd_lem = Q.store_thm("nfst_nsnd_lem",
@@ -814,21 +768,4 @@ val NSND_ENCODE_TM_TAPE_DIV2 = Q.store_thm("NSND_ENCODE_TM_TAPE_DIV2[simp]",
 `(nsnd (ENCODE_TM_TAPE tm) DIV 2) = ENCODE tm.tape_r`,
 rw[ENCODE_TM_TAPE_def])
 
-val ENCODE_ZERO_NONEMPTY = Q.store_thm("ENCODE_ZERO_NONEMPTY",
-`((ENCODE t = 0) ∧ ¬(t=[])) ==> (HD t = Z)`,
-Cases_on `t` >> fs[] >>fs[ENCODE_def]  >> Cases_on `h` >> fs[])
-
-
-val ENCODE_TL_ZERO = Q.store_thm("ENCODE_TL_ZERO",
-`¬(t = []) ==> ((ENCODE t = 0) ==> (ENCODE (TL t) = 0))`,
-Cases_on `t` >> fs[] >>fs[ENCODE_def]  >> Cases_on `h` >> fs[])
-
-
-
 val _ = export_theory();
-
-
-
-
-
-
